PhysLean/StringTheory/FTheory/SU5/Quanta/FiveQuanta.lean
@@ -4,7 +4,6 @@ Released under Apache 2.0 license as described in the file LICENSE.
 Authors: Joseph Tooby-Smith
 -/
 import PhysLean.StringTheory.FTheory.SU5.Fluxes.NoExotics.ToList
-import PhysLean.Particles.SuperSymmetry.SU5.Charges.MinimallyAllowsTerm.OfFinset
 import PhysLean.StringTheory.FTheory.SU5.Charges.OfRationalSection
 import PhysLean.Particles.SuperSymmetry.SU5.Charges.Map
 /-!
